形如：

$F(x)=\int_{c(x)}^{d(x)}f(x,y)\mathrm{d}y$

其微分为：

$\frac{\mathrm{d}}{\mathrm{d}x}\int_{c(x)}^{d(x)}f(x,y)\mathrm{d}y=f(x,d(x))d'(x)-f(x,c(x))c'(x)+\int_{c(x)}^{d(x)}f'(x,y)\mathrm{d}y$

证明：

设$H(x,c,d)=\int_{c}^{d}f(x,y)\mathrm{d}y$，则$F(x)=H(x,c(x),d(x))$. 

$F'(x) =\frac{\partial H}{\partial x}+\frac{\partial H}{\partial c}c'(x)+\frac{\partial H}{\partial d}d'(x)$
     $=\int_{c(x)}^{d(x)}f'_{x}(x,y)\mathrm{d}y-f(x,c(x))c'(x)+f(x,d(x))d'(x)$
     $=f(x,d(x))d'(x)-f(x,c(x))c'(x)+\int_{c(x)}^{d(x)}f'(x,y)\mathrm{d}y$
														$\Box$
