
## 递推1

$$
C_{n+1}^{m+1}=C_{n}^{m+1}+C_{n}^{m}
$$
或
$$
C_{n}^{m}=C_{n+1}^{m+1}-C_{n}^{m+1}
$$
则
$$
\begin{align} \\
 \\

&\sum_{k=m}^{n} C_{k}^{m} \\
&=\sum_{k=m}^{n}C_{k+1}^{m+1}-C_{k}^{m+1}\\
 &=C_{n+1}^{m+1}-C_{m+1}^{m+1}+C_{m}^{m}\\
&=C_{n+1}^{m+1}
\end{align}
$$\


## 递推2

$$

mC_{n}^{m}=\frac{n!}{m!(n-m)!}=n \frac{(n-1)!}{(m-1)!(n-m)!}=nC_{n-1}^{m-1}
$$


即
$$
C_{n}^{m}=\frac{n}{m}C_{n-1}^{m-1}
$$


## 范德蒙恒等式

考虑超几何分布：$$
P(X=m)=\frac{C_{M}^{m}C_{N-M}^{n-m}}{C_{N}^{n}},m=0,1,\dots,n 
$$
有
$$

\sum_{m=0}^{n}P(X=m)=\sum_{m=0}^{n} \frac{C_{M}^{m}C_{N-M}^{n-m}}{C_{N}^{n}}=1


$$

即
$$
C_{n+m}^{k}=\sum_{i=0}^{k} C_{n}^{i}C_{m}^{k-i}
$$


