
进行n次实验，每次成功的概率是p，每次实验相互独立，计X为n次实验中成功的次数，则X的概率分布：

$$
P(X=m)=C_{n}^{m}p^m(1-p)^{n-m},m=0,1,\dots,n
$$
记为$B(n,p)$.

### 期望

$$
\begin{align}

&E(X)=\sum_{m=0}^{n} mP(X=m) \\
&=\sum_{m=0}^{n}mC_{n}^{m}p^m(1-p)^{n-m} \\
&=\sum_{m=1}^{n}mC_{n}^{m}p^m(1-p)^{n-m} \\
&=\sum_{m=1}^{n}nC_{n-1}^{m-1}p^{m}(1-p)^{n-m}  \\ 
&=\sum_{m=0}^{n-1}nC_{n-1}^{m}p^{m+1}(1-p)^{n-m-1}  \\ 
&=np\sum_{m=0}^{n-1}C_{n-1}^{m}p^{m}(1-p)^{n-m-1}  \\ 
&=np
\end{align}
$$

### 方差

$$
\begin{align}

&E(X^{2})=\sum_{m=0}^{n} m^{2}P(X=m) \\
&=\sum_{m=1}^{n}m^{2}C_{n}^{m}p^m(1-p)^{n-m}  \\
&=\sum_{m=1}^{n}nmC_{n-1}^{m-1}p^{m}(1-p)^{n-m}  \\ 
&=\sum_{m=0}^{n-1}n(m+1)C_{n-1}^{m}p^{m+1}(1-p)^{n-m-1}   \\
&=\sum_{m=0}^{n-1}nC_{n-1}^{m}p^{m+1}(1-p)^{n-m-1}  \\
&+\sum_{m=0}^{n-1}nmC_{n-1}^{m}p^{m+1}(1-p)^{n-m-1}  \\ 
&=np+np\sum_{m=0}^{n-1}mC_{n-1}^{m}p^{m}(1-p)^{n-m-1}   \\
&=np+np(n-1)p \\
&=np((n-1)p+1)  \\

\end{align}


$$

$$
\begin{align}
&D(X)=E(X^{2})-[E(X)]^{2}  \\
&=np((n-1)p+1)-(np)^{2} \\
&=np(1-p)
\end{align}
$$


